Dependent Records In Progress

Arm.v
@@ -53,13 +53,6 @@ Definition is_ra l := match l with
                         | R_Acq _ _    => True
                       end.
 
-(* ARM axiom *)
-(* bob = ((R_acq_pc ; po) ∪ (po ; W_rel)) *)
-(* intervening-write(rel) = rel ; W ; rel *)
-(* lrs = W ; poloc / intervening-write(poloc) ; R *)
-(* aob = rmw ∪ (W ∩ codomain(rmw) ; lrs ; R) *)
-(* ob = (bob ∪ aob U rfe ∪ moe ∪ fre)+ *)
-
 Definition R: relation Event := ⦗fun r => is_r (event_label r)⦘.
 Definition W: relation Event := ⦗fun w => is_w (event_label w)⦘.
 Definition RA: relation Event := ⦗fun r => is_ra (event_label r)⦘. 
@@ -88,40 +81,48 @@ Definition ob (exec: Execution): relation Event :=
 Definition ordered_before_axiom_arm (exec: Execution): Prop := 
     irreflexive (ob exec).
 
-Definition arm_consistent (exec: Execution): Prop := 
-    well_formed exec /\ (amo exec) ≡ (rmw exec) /\ atomicity_axiom exec /\ coherence_axiom exec /\ ordered_before_axiom_arm exec.
+Record ArmConsistent (exec: Execution) := {
+    ac_amo  : (amo exec) ≡ (rmw exec); 
+    ac_atom : atomicity_axiom exec; 
+    ac_coh  : coherence_axiom exec; 
+    ac_ob   : ordered_before_axiom_arm exec
+}.  
 
-Lemma same_thread_dec_arm:
-    forall (e1 e2 : @Event LabelArm LabelClassArm),
+Record ArmConsistentExecution: Type := {
+    exec_arm :> @WellFormedExecution LabelArm LabelClassArm; 
+    arm_cons: ArmConsistent exec_arm; 
+}.
+
+Lemma same_thread_dec_arm: forall (e1 e2: Event),
     {same_thread e1 e2} + {~ same_thread e1 e2}.
 Proof with eauto.
     intros e1 e2.
-    destruct e1; destruct e2; simpl.
-    - right...
-    - right...
-    - right...
-    - destruct (Nat.eq_dec tid tid0).
-      + left...
-      + right...
+    destruct e1; destruct e2; simpl. all:try(eauto).  
+    destruct (Nat.eq_dec tid tid0); eauto. 
 Qed.
 
-Lemma arm_consistent_amo_is_rmw: 
-    forall (execArm: @Execution LabelArm LabelClassArm) (e0 e1: @Event LabelArm LabelClassArm),
-        (amo execArm) ≡ (rmw execArm) -> (rmw execArm) e0 e1 -> (amo execArm) e0 e1.
+Lemma arm_consistent_amo_is_rmw: forall (execArm: Execution) (e0 e1: Event),
+        (amo execArm) ≡ (rmw execArm) -> 
+            (rmw execArm) e0 e1 
+                -> (amo execArm) e0 e1.
 Proof with eauto. 
     intros.
     unfold same_relation in *. destruct H as [Hamo Hrmw]. 
     unfold inclusion in *...      
 Qed.
 
-Lemma po_in_events_l : forall (execArm : @Execution LabelArm LabelClassArm) x y,
-    well_formed_po execArm -> po execArm x y ->  events execArm x.
+Lemma po_in_events_l : forall (execArm: Execution) x y,
+    well_formed_po execArm -> 
+        po execArm x y ->  
+            events execArm x.
 Proof with eauto.
     intros. unfold well_formed_po in *. destruct H as [H1 H2]. apply H1 in H0. destruct H0 as [H0 _]...
 Qed.
 
-Lemma po_in_events_r : forall (execArm : @Execution LabelArm LabelClassArm) x y,
-    well_formed_po execArm -> po execArm x y -> events execArm y.
+Lemma po_in_events_r : forall (execArm: Execution) x y,
+    well_formed_po execArm -> 
+        po execArm x y -> 
+            events execArm y.
 Proof with eauto.
     intros. unfold well_formed_po in *. destruct H as [H1 H2]. apply H1 in H0. destruct H0 as [_ H0]...
 Qed.  
